trials on sem_eq and sem_eq_k definition

eqqq.thy
@@ -7,9 +7,9 @@ typedecl TreeHandle
 datatype ThunkHandle = HThunkHandle TreeHandle
 
 datatype handle = 
-HBlobHandle BlobHandle
-| HTreeHandle TreeHandle
-| HThunkHandle ThunkHandle
+  HBlobHandle BlobHandle
+  | HTreeHandle TreeHandle
+  | HThunkHandle ThunkHandle
 
 typedecl raw
 type_synonym BlobData = "raw"
@@ -22,9 +22,9 @@ consts
   get_tree_raw :: "TreeHandle \<Rightarrow> handle list"
   get_thunk_tree :: "ThunkHandle \<Rightarrow> TreeHandle"
 
-  create_blob :: "BlobData \<Rightarrow> BlobHandle"
-  create_tree :: "TreeData \<Rightarrow> TreeHandle"
-  create_thunk :: "TreeHandle \<Rightarrow> ThunkHandle"
+create_blob :: "BlobData \<Rightarrow> BlobHandle"
+create_tree :: "TreeData \<Rightarrow> TreeHandle"
+create_thunk :: "TreeHandle \<Rightarrow> ThunkHandle"
 
 definition get_tree_data :: "TreeHandle \<Rightarrow> nat \<Rightarrow> handle" where
   "get_tree_data t i \<equiv> (get_tree_raw t) ! i"
@@ -32,16 +32,21 @@ definition get_tree_data :: "TreeHandle \<Rightarrow> nat \<Rightarrow> handle" 
 definition get_tree_size :: "TreeHandle \<Rightarrow> nat" where
   "get_tree_size t \<equiv> length (get_tree_raw t)"
 
+fun get_type :: "handle \<Rightarrow> nat" where
+  "get_type (HBlobHandle _ ) = 0"
+| "get_type (HTreeHandle _ ) = 1"
+| "get_type (HThunkHandle _ ) = 2"
+
 (* User Program *)
 
 datatype op =
-     OGetBlobData nat
-   | OGetTreeData nat nat
-   | OCreateBlob nat
-   | OCreateTree "nat list"
-   | OCreateThunk nat
-   | ORunInternal
-   | OReturn nat
+  OGetBlobData nat
+  | OGetTreeData nat nat
+  | OCreateBlob nat
+  | OCreateTree "nat list"
+  | OCreateThunk nat
+  | ORunInternal
+  | OReturn nat
 
 record state =
   hs :: "handle list"
@@ -82,35 +87,35 @@ datatype step_result =
 
 inductive step :: "op \<Rightarrow> state \<Rightarrow> step_result \<Rightarrow> bool"
   where
-StepGetBlobData:
+    StepGetBlobData:
     "i < length (hs s) \<Longrightarrow> hs s ! i = HBlobHandle b \<Longrightarrow>
     step (OGetBlobData i) s (Continue (dpush s (get_blob_data b)))"
 
 | StepGetTreeData:
-    "i < length (hs s) \<Longrightarrow> 
+  "i < length (hs s) \<Longrightarrow> 
      hs s ! i = HTreeHandle t \<Longrightarrow>
      j < get_tree_size t \<Longrightarrow>
     step (OGetTreeData i j) s (Continue (hpush s (get_tree_data t j)))"
 
 | StepCreateBlob:
-    "i < length (ds s) \<Longrightarrow> 
+  "i < length (ds s) \<Longrightarrow> 
     step (OCreateBlob i) s (Continue (hpush s (HBlobHandle (create_blob (ds s ! i)))))"
 
 | StepCreateThunk:
-    "i < length (hs s) \<Longrightarrow> hs s ! i = HTreeHandle t \<Longrightarrow>
+  "i < length (hs s) \<Longrightarrow> hs s ! i = HTreeHandle t \<Longrightarrow>
     step (OCreateThunk i) s (Continue (hpush s (HThunkHandle (create_thunk t))))"
 
 | StepCreateTree:
-    "\<forall>i\<in>set xs. i < length (hs s) \<Longrightarrow>
+  "\<forall>i\<in>set xs. i < length (hs s) \<Longrightarrow>
      hlist = map (\<lambda>i. hs s ! i) xs \<Longrightarrow>
      step (OCreateTree xs) s (Continue (hpush s (HTreeHandle (create_tree hlist) )))" 
 
 | StepReturn:
-    "i < length (hs s) \<Longrightarrow> r = hs s ! i \<Longrightarrow>
+  "i < length (hs s) \<Longrightarrow> r = hs s ! i \<Longrightarrow>
     step (OReturn i) s (Return (hs s ! i))"
 
 | StepRunInternal:
-    "step ORunInternal s (Continue (run_internal s))"
+  "step ORunInternal s (Continue (run_internal s))"
 
 fun step_fun :: "op \<Rightarrow> state \<Rightarrow> step_result option" where
   "step_fun (OGetBlobData i) s = 
@@ -148,15 +153,15 @@ fun step_fun :: "op \<Rightarrow> state \<Rightarrow> step_result option" where
 
 inductive exec :: "userprog \<Rightarrow> state \<Rightarrow> handle \<Rightarrow> bool"
   where
-  ExecReturn:
+    ExecReturn:
     "step i s (Return r) \<Longrightarrow> exec (i # xs) s r"
-| ExecStep:
+  | ExecStep:
     "step i s (Continue s') \<Longrightarrow> exec xs s' r \<Longrightarrow> exec (i # xs) s r"
 
 fun exec_fun :: "userprog \<Rightarrow> state \<Rightarrow> handle option"
   where
-  "exec_fun [] s = None"
-| "exec_fun (i # xs) s =
+    "exec_fun [] s = None"
+  | "exec_fun (i # xs) s =
    (case (step_fun i s) of
    None \<Rightarrow> None
    | Some (Return r) \<Rightarrow> Some r
@@ -174,17 +179,17 @@ fun is_thunk :: "handle \<Rightarrow> bool" where
   "is_thunk (HThunkHandle _) = True"
 | "is_thunk _ = False"
 
-inductive evaluate_with_fuel :: "nat \<Rightarrow> handle \<Rightarrow> handle \<Rightarrow> bool" where
+inductive force_with_fuel :: "nat \<Rightarrow> handle \<Rightarrow> handle \<Rightarrow> bool" where
   Done:
-    "\<not> is_thunk h \<Longrightarrow> evaluate_with_fuel n h h"
+  "\<not> is_thunk h \<Longrightarrow> force_with_fuel n h h"
 | Step:
-    "h = HThunkHandle thunk \<Longrightarrow>
+  "h = HThunkHandle thunk \<Longrightarrow>
      Some h1 = apply_thunk thunk \<Longrightarrow>
-     evaluate_with_fuel n h1 h2 \<Longrightarrow>
-     evaluate_with_fuel (Suc n) h h2"
+     force_with_fuel n h1 h2 \<Longrightarrow>
+     force_with_fuel (Suc n) h h2"
 
-fun evaluate_with_fuel_fun :: "nat \<Rightarrow> handle \<Rightarrow> handle option" where
-  "evaluate_with_fuel_fun n h =
+fun force_with_fuel_fun :: "nat \<Rightarrow> handle \<Rightarrow> handle option" where
+  "force_with_fuel_fun n h =
      (case h of
         HThunkHandle th \<Rightarrow>
           (case n of
@@ -192,11 +197,11 @@ fun evaluate_with_fuel_fun :: "nat \<Rightarrow> handle \<Rightarrow> handle opt
            | Suc n' \<Rightarrow>
                (case apply_thunk th of
                   None \<Rightarrow> None
-                | Some h1 \<Rightarrow> evaluate_with_fuel_fun n' h1))
+                | Some h1 \<Rightarrow> force_with_fuel_fun n' h1))
        | _ \<Rightarrow> Some h)"
 
-definition evaluates_to :: "handle \<Rightarrow> handle \<Rightarrow> bool" where
-  "evaluates_to h h1 \<equiv> (\<exists>fuel. evaluate_with_fuel_fun fuel h = Some h1 \<and> \<not> is_thunk h1)"
+definition forces_to :: "handle \<Rightarrow> handle \<Rightarrow> bool" where
+  "forces_to h h1 \<equiv> (\<exists>fuel. force_with_fuel_fun fuel h = Some h1 \<and> \<not> is_thunk h1)"
 
 (* Determinism *)
 
@@ -207,7 +212,7 @@ lemma step_deterministic:
 proof (induction arbitrary: o2 rule: step.induct)
   case (StepGetBlobData i s b)
   from StepGetBlobData.prems(1) show ?case
-  by (cases rule: step.cases; auto simp: StepGetBlobData(2))
+    by (cases rule: step.cases; auto simp: StepGetBlobData(2))
 next
   case (StepGetTreeData i s b j)
   from StepGetTreeData.prems(1) show ?case
@@ -242,7 +247,7 @@ proof (induction arbitrary: o2 rule: exec.induct)
   case (ExecReturn i s r1 xs)
   then show ?case
     by (cases rule: exec.cases[OF ExecReturn.prems(1)])
-       (auto dest: step_deterministic)
+      (auto dest: step_deterministic)
 next
   case (ExecStep i s s' xs r)
   have H1: "step i s (Continue s')" using ExecStep.hyps(1) by assumption
@@ -265,19 +270,19 @@ next
   qed
 qed
 
-lemma evaluate_with_fuel_deterministic:
-  assumes A: "evaluate_with_fuel n h r1"
-      and B: "evaluate_with_fuel n h r2"
+lemma force_with_fuel_deterministic:
+  assumes A: "force_with_fuel n h r1"
+    and B: "force_with_fuel n h r2"
   shows "r1 = r2"
-using A B
-proof (induction arbitrary: r2 rule: evaluate_with_fuel.induct)
+  using A B
+proof (induction arbitrary: r2 rule: force_with_fuel.induct)
   case (Done h n)
   then show ?case
-    by (cases rule: evaluate_with_fuel.cases[OF Done.prems]) auto
+    by (cases rule: force_with_fuel.cases[OF Done.prems]) auto
 next
   case (Step h thunk h1 n h2)
   then show ?case
-  proof (cases rule: evaluate_with_fuel.cases[OF Step.prems])
+  proof (cases rule: force_with_fuel.cases[OF Step.prems])
     case (1 ha na)
     have A: "\<not> is_thunk h" using 1(4) 1(2) by auto
     have B: "is_thunk h" using local.Step(1) by auto
@@ -288,20 +293,20 @@ next
     then have "apply_thunk thunka = apply_thunk thunk" by auto
     then have "Some h1a = Some h1" using 2(5) Step.hyps(2) by simp
     then have "h1a = h1" by simp
-    then have "evaluate_with_fuel n h1 h2a" using 2(1) 2(6) by auto
+    then have "force_with_fuel n h1 h2a" using 2(1) 2(6) by auto
     thus ?thesis using Step.IH 2(3) by auto
   qed
 qed
 
 lemma evaluate_with_fuel_pad:
-  assumes "evaluate_with_fuel f h nf" and "\<not> is_thunk nf"
-  shows "evaluate_with_fuel (f + k) h nf"
+  assumes "force_with_fuel f h nf" and "\<not> is_thunk nf"
+  shows "force_with_fuel (f + k) h nf"
   using assms
-  by (induction rule: evaluate_with_fuel.induct) (simp_all add: evaluate_with_fuel.intros)
+  by (induction rule: force_with_fuel.induct) (simp_all add: force_with_fuel.intros)
 
-lemma evaluate_with_fuel_fun_pad:
-  assumes "evaluate_with_fuel_fun f h = Some h1" and "\<not> is_thunk h1"
-  shows "evaluate_with_fuel_fun (f + k) h = Some h1"
+lemma force_with_fuel_fun_pad:
+  assumes "force_with_fuel_fun f h = Some h1" and "\<not> is_thunk h1"
+  shows "force_with_fuel_fun (f + k) h = Some h1"
   using assms
 proof (induction f arbitrary: h)
   case 0 then show ?case by (cases h) auto
@@ -310,133 +315,255 @@ next
   then show ?case 
   proof (cases h) 
     case (HBlobHandle b)
-    then have "evaluate_with_fuel_fun (Suc f') h = Some h" by simp_all
+    then have "force_with_fuel_fun (Suc f') h = Some h" by simp_all
     then have "h1 = h" using Suc.prems(1) by auto
     then show ?thesis using HBlobHandle by auto
   next
     case (HTreeHandle t)
-    then have "evaluate_with_fuel_fun (Suc f') h = Some h" by simp_all
+    then have "force_with_fuel_fun (Suc f') h = Some h" by simp_all
     then have "h1 = h" using Suc.prems(1) by auto
     then show ?thesis using HTreeHandle by auto
   next
     case (HThunkHandle th)
     from Suc.prems(1) HThunkHandle obtain h2 where
       A: "apply_thunk th = Some h2"
-      and B: "evaluate_with_fuel_fun f' h2 = Some h1" by (simp split: option.splits)
+      and B: "force_with_fuel_fun f' h2 = Some h1" by (simp split: option.splits)
 
-    have "evaluate_with_fuel_fun (f' + k) h2 = Some h1" using B Suc.IH Suc.prems(2) by auto
+    have "force_with_fuel_fun (f' + k) h2 = Some h1" using B Suc.IH Suc.prems(2) by auto
     then show ?thesis using HThunkHandle A by simp_all
   qed
 qed
 
-theorem evaluates_to_deterministic:
-  assumes "evaluates_to h h1" and "evaluates_to h h2"
+lemma forces_to_deterministic:
+  assumes "forces_to h h1" and "forces_to h h2"
   shows "h1 = h2"
   using assms
 proof -
-  obtain f1 where A: "evaluate_with_fuel_fun f1 h = Some h1" and NT1: "\<not> is_thunk h1"
-    using assms(1) unfolding evaluates_to_def by auto
-  obtain f2 where B: "evaluate_with_fuel_fun f2 h = Some h2" and NT2: "\<not> is_thunk h2"
-    using assms(2) unfolding evaluates_to_def by auto
+  obtain f1 where A: "force_with_fuel_fun f1 h = Some h1" and NT1: "\<not> is_thunk h1"
+    using assms(1) unfolding forces_to_def by auto
+  obtain f2 where B: "force_with_fuel_fun f2 h = Some h2" and NT2: "\<not> is_thunk h2"
+    using assms(2) unfolding forces_to_def by auto
   let ?F = "max f1 f2"
   let ?k1 = "?F - f1"
   let ?k2 = "?F - f2"
-  have "evaluate_with_fuel_fun (f1 + ?k1) h = Some h1"
-    using evaluate_with_fuel_fun_pad[OF A NT1] .
-  then have AA: "evaluate_with_fuel_fun ?F h = Some h1" by simp
-  have "evaluate_with_fuel_fun (f2 + ?k2) h = Some h2" 
-    using evaluate_with_fuel_fun_pad[OF B NT2] .
-  then have BB: "evaluate_with_fuel_fun ?F h = Some h2" by simp
+  have "force_with_fuel_fun (f1 + ?k1) h = Some h1"
+    using force_with_fuel_fun_pad[OF A NT1] .
+  then have AA: "force_with_fuel_fun ?F h = Some h1" by simp
+  have "force_with_fuel_fun (f2 + ?k2) h = Some h2" 
+    using force_with_fuel_fun_pad[OF B NT2] .
+  then have BB: "force_with_fuel_fun ?F h = Some h2" by simp
   show ?thesis using AA BB by simp
+qed
+
+lemma forces_to_not_thunk:
+  assumes "forces_to h h1"
+  shows "\<not> is_thunk h1"
+  using assms
+  unfolding forces_to_def
+  by auto
+
+definition force :: "handle \<Rightarrow> handle option" where
+  "force h =
+     (if (\<exists>v. forces_to h v)
+      then Some (THE v. forces_to h v)
+      else None)"
+
+lemma force_some:
+  assumes "force h = Some h1"
+  shows "forces_to h h1"
+  using assms
+  unfolding force_def
+proof -
+  have ex: "\<exists>x. forces_to h x"
+    using assms unfolding force_def by (auto split: if_splits)
+  have ex1: "\<exists>!x. forces_to h x"
+    using ex forces_to_deterministic by (auto)
+  have "forces_to h (THE x. forces_to h x)"
+    using ex1 by (rule theI')
+  moreover have "h1 = (THE x. forces_to h x)"
+    using assms ex unfolding force_def by (auto split: if_splits)
+  ultimately show ?thesis by simp
+qed
+
+lemma force_unique:
+  assumes "forces_to h h1"
+  shows "force h = Some h1"
+  using assms
+proof -
+  have ex: "\<exists>x. forces_to h x" using assms by blast
+  have ex1: "\<exists>!y. forces_to h y"
+    using assms forces_to_deterministic by auto
+  have the_eq: "(THE x. forces_to h x) = h1"
+    using assms ex1 by auto
+  show ?thesis
+    unfolding force_def using ex the_eq by simp
 qed
 
 (* Blob/Tree creation rules *)
 
 axiomatization where
   get_blob_data_create_blob[simp]:
-    "get_blob_data (create_blob x) = x"
-and
+  "get_blob_data (create_blob x) = x"
+  and
   get_tree_raw_create_tree[simp]:
-    "get_tree_raw (create_tree xs) = xs"
-and
+  "get_tree_raw (create_tree xs) = xs"
+  and
   get_thunk_tree_create_thunk[simp]:
-    "get_thunk_tree (create_thunk t) = t"
+  "get_thunk_tree (create_thunk t) = t"
 
 (* Coupon rules *)
 
 inductive coupon_eq :: "handle \<Rightarrow> handle \<Rightarrow> bool" where
   Storage:
-    "get_blob_data h1 = get_blob_data h2 \<Longrightarrow> coupon_eq (HBlobHandle h1) (HBlobHandle h2)"
+  "get_blob_data h1 = get_blob_data h2 \<Longrightarrow> coupon_eq (HBlobHandle h1) (HBlobHandle h2)"
 | Tree:
-    "get_tree_size t1 = get_tree_size t2 \<Longrightarrow>
+  "get_tree_size t1 = get_tree_size t2 \<Longrightarrow>
      (\<forall> i < get_tree_size t1. coupon_eq (get_tree_data t1 i) (get_tree_data t2 i)) \<Longrightarrow>
      coupon_eq (HTreeHandle t1) (HTreeHandle t2)"
 | ThunkByTree:
-    "coupon_eq (HTreeHandle (get_thunk_tree th1)) (HTreeHandle (get_thunk_tree th2)) \<Longrightarrow>
+  "coupon_eq (HTreeHandle (get_thunk_tree th1)) (HTreeHandle (get_thunk_tree th2)) \<Longrightarrow>
      coupon_eq (HThunkHandle th1) (HThunkHandle th2)"
 | ThunkByEvaluate:
-    "evaluates_to (HThunkHandle th1) h \<Longrightarrow>
-     evaluates_to (HThunkHandle th2) h \<Longrightarrow>
+  "forces_to (HThunkHandle th1) h \<Longrightarrow>
+     forces_to (HThunkHandle th2) h \<Longrightarrow>
      coupon_eq (HThunkHandle th1) (HThunkHandle th2)"
 
 (* Semantic rules *)
 
-inductive sem_eq :: "handle \<Rightarrow> handle \<Rightarrow> bool" where
- SemBlob:
+coinductive sem_eq :: "handle \<Rightarrow> handle \<Rightarrow> bool" where
+  SemBlob:
   "(get_blob_data b1 = get_blob_data b2) \<Longrightarrow> sem_eq (HBlobHandle b1) (HBlobHandle b2)"
 | SemTree:
-  "get_tree_size t1 = get_tree_size t2 \<Longrightarrow>
-   (\<forall>i < get_tree_size t1. sem_eq (get_tree_data t1 i) (get_tree_data t2 i)) \<Longrightarrow>
+  "list_all2 sem_eq (get_tree_raw t1) (get_tree_raw t2) \<Longrightarrow>
    sem_eq (HTreeHandle t1) (HTreeHandle t2)"
 | SemThunk:
-  "(\<forall>r1 r2.
-     evaluates_to (HThunkHandle th1) r1 \<Longrightarrow>
-     evaluates_to (HThunkHandle th2) r2 \<Longrightarrow>
+  "(force (HThunkHandle th1) = Some r1 \<Longrightarrow>
+    force (HThunkHandle th2) = Some r2 \<Longrightarrow>
      sem_eq r1 r2) \<Longrightarrow>
    sem_eq (HThunkHandle th1) (HThunkHandle th2)"
 
+coinductive sem_eq_k :: "nat \<Rightarrow> handle \<Rightarrow> handle \<Rightarrow> bool" where
+  SemBlob:
+  "(get_blob_data b1 = get_blob_data b2) \<Longrightarrow> sem_eq_k k (HBlobHandle b1) (HBlobHandle b2)"
+| SemTree:
+  "list_all2 sem_eq (get_tree_raw t1) (get_tree_raw t2) \<Longrightarrow>
+   sem_eq_k k (HTreeHandle t1) (HTreeHandle t2)"
+| SemThunk0:
+  "sem_eq_k 0 (HThunkHandle th1) (HThunkHandle th2)"
+| SemThunkk:
+  "(force (HThunkHandle th1) = Some r1 \<Longrightarrow>
+    force (HThunkHandle th2) = Some r2 \<Longrightarrow>
+     sem_eq_k k r1 r2) \<Longrightarrow>
+   sem_eq_k (Suc k) (HThunkHandle th1) (HThunkHandle th2)"
 
+lemma sem_eq_same_type:
+  assumes "sem_eq h1 h2"
+  shows "get_type h1 = get_type h2"
+  using assms
+  by (cases rule: sem_eq.cases) auto
 
-    
-     
+(* sem_eq preserved by thunk application *)
 
-
-
-
-section "Useful lemmas"
-
+(* 1. Useful lemmas and definitions *)
 definition relate_opt :: "('a \<Rightarrow> 'b \<Rightarrow> bool) \<Rightarrow> 'a option \<Rightarrow> 'b option \<Rightarrow> bool" where
   "relate_opt P x y \<equiv>
      (case x of None \<Rightarrow> y = None 
      | Some a \<Rightarrow> (\<exists>b. y = Some b \<and> P a b))"
 
-definition relate_state :: "(handle\<times>handle) set \<Rightarrow> state \<Rightarrow> state \<Rightarrow> bool" where
-  "relate_state R s1 s2 \<equiv>
-     list_all2 (\<lambda>h1 h2. (h1,h2) \<in> R) (hs s1) (hs s2) \<and> ds s1 = ds s2"
-
-lemma relate_state_append_d:
-  assumes "relate_state R u1 u2" and "d1 = d2"
-  shows "relate_state R (u1 \<lparr>ds := ds u1 @ [d1]\<rparr>) (u2 \<lparr>ds := ds u2 @ [d2]\<rparr>)"
-  using assms unfolding relate_state_def by auto
+definition sem_eq_state :: "state \<Rightarrow> state \<Rightarrow> bool" where
+  "sem_eq_state s1 s2 \<equiv>
+     list_all2 (\<lambda>h1 h2. sem_eq h1 h2) (hs s1) (hs s2) \<and> ds s1 = ds s2"
 
 lemma list_all2_append:
   assumes "list_all2 P xs ys"
-      and "P x y"
+    and "P x y"
   shows   "list_all2 P (xs @ [x]) (ys @ [y])"
-using assms
-proof (induction arbitrary: x y rule: list_all2_induct)
-  case Nil
-  then show ?case by simp
-next
-  case (Cons a xs b ys)
-  then show ?case by simp
+  using assms
+  by (induction arbitrary: x y rule: list_all2_induct) simp_all
+
+lemma list_all2_nthD:
+  assumes "list_all2 R xs ys" "i < length xs"
+  shows "i < length ys \<and> R (xs ! i) (ys ! i)"
+  using assms
+  by (auto simp: list_all2_conv_all_nth)
+
+lemma sem_eq_state_hpush:
+  assumes "sem_eq_state s1 s2" and "sem_eq h1 h2"
+  shows "sem_eq_state (hpush s1 h1) (hpush s2 h2)"
+  using assms unfolding sem_eq_state_def hpush_def
+  by (auto simp: list_all2_append)
+
+lemma sem_eq_dpush:
+  assumes "sem_eq_state s1 s2" and "d1 = d2"
+  shows "sem_eq_state (dpush s1 d1) (dpush s2 d2)"
+  using assms unfolding sem_eq_state_def dpush_def by auto
+
+lemma sem_eq_same_kind:
+  assumes "sem_eq h1 h2"
+  shows
+    "(\<exists>b1 b2. h1 = HBlobHandle b1 \<and> h2 = HBlobHandle b2) \<or>
+     (\<exists>t1 t2. h1 = HTreeHandle t1 \<and> h2 = HTreeHandle t2) \<or>
+     (\<exists>k1 k2. h1 = HThunkHandle k1 \<and> h2 = HThunkHandle k2)"
+  using assms
+  by (cases rule: sem_eq.cases) auto
+
+definition rel_step_result :: "step_result \<Rightarrow> step_result \<Rightarrow> bool" where
+  "rel_step_result r1 r2 \<equiv> 
+   (case (r1, r2) of
+     (Continue s1, Continue s2) \<Rightarrow> sem_eq_state s1 s2
+   | (Return r1, Return r2) \<Rightarrow> sem_eq r1 r2
+   | (_, _) \<Rightarrow> False)"
+
+(* 2. API functions respect sem_eq *)
+lemma get_blob_data_sem_eq:
+  assumes "sem_eq (HBlobHandle b1) (HBlobHandle b2)"
+  shows "get_blob_data b1 = get_blob_data b2"
+  using assms
+  by (cases rule: sem_eq.cases) auto
+
+lemma sem_eq_tree_children:
+  assumes "sem_eq (HTreeHandle t1) (HTreeHandle t2)"
+  shows "list_all2 sem_eq (get_tree_raw t1) (get_tree_raw t2)"
+  using assms
+  by (cases rule: sem_eq.cases) auto
+
+lemma get_tree_size_sem_eq:
+  assumes "sem_eq (HTreeHandle t1) (HTreeHandle t2)"
+  shows   "get_tree_size t1 = get_tree_size t2"
+  using sem_eq_tree_children[OF assms]
+  by (simp add: get_tree_size_def list_all2_lengthD)
+
+lemma get_tree_data_sem_eq:
+  assumes "sem_eq (HTreeHandle t1) (HTreeHandle t2)" and "i < get_tree_size t1"
+  shows "sem_eq (get_tree_data t1 i) (get_tree_data t2 i)"
+proof -
+  have A: "i < length (get_tree_raw t1)" using assms(2) get_tree_size_def by auto
+  have "list_all2 sem_eq (get_tree_raw t1) (get_tree_raw t2)" 
+    using sem_eq_tree_children[OF assms(1)] .
+  then have "sem_eq ((get_tree_raw t1) ! i) ((get_tree_raw t2) ! i)" 
+    using list_all2_nthD[OF _ A] by auto
+  then show ?thesis by (simp add: get_tree_data_def[symmetric]) 
 qed
 
-lemma relate_ustate_append_h:
-  assumes "relate_state R u1 u2" and "(h1,h2) \<in> R"
-  shows "relate_state R (u1 \<lparr>hs := hs u1 @ [h1]\<rparr>) (u2 \<lparr>hs := hs u2 @ [h2]\<rparr>)"
-  using assms unfolding relate_state_def
-  by (auto simp: list_all2_append)
+lemma create_blob_sem_eq:
+  assumes "d1 = d2"
+  shows "sem_eq (HBlobHandle (create_blob d1)) (HBlobHandle (create_blob d2))"
+proof -
+  have "get_blob_data (create_blob d1) = get_blob_data (create_blob d2)" 
+    using assms by simp_all
+  then show ?thesis by (rule sem_eq.SemBlob) 
+qed
+
+lemma create_tree_sem_eq:
+  assumes "list_all2 sem_eq xs ys"
+  shows "sem_eq (HTreeHandle (create_tree xs)) (HTreeHandle (create_tree ys))"
+proof -
+  have "list_all2 sem_eq (get_tree_raw (create_tree xs)) (get_tree_raw (create_tree ys))"
+    using assms by simp_all
+  then show ?thesis by (rule sem_eq.SemTree)
+qed
+
+
 
 
 
